lemmas, replaced some ssr predicates with stdpp ones

theories/iris.v
@@ -34,7 +34,7 @@ Definition val := list value.
 Definition state : Type := host_state * store_record.
 Definition observation := unit. (* TODO: maybe change? *)
 
-Definition of_val (v : val) : expr := map (fun v => AI_basic (BI_const v)) v.
+Definition of_val (v : val) : expr := fmap (fun v => AI_basic (BI_const v)) v.
 
 Fixpoint to_val (e : expr) : option val :=
   match e with
